


Acquisition fn $\alpha(x)$

- Depends on past info (implicit)
- Sample location x

$\alpha(x)$ in simple EI case is

$$\mathbb{E} [(f(x) - f_*)_+]$$

↑
random piece, 1D Gaussian
Compute integral in "closed form"

Want to optimize via gradient descent

General: $\alpha(x) = \mathbb{E}[g(x)]$

$$\nabla \alpha(x) = \mathbb{E}[\nabla g(x)]$$

(with enough reg.)

$$\hat{\alpha}(x) = \frac{1}{N} \sum_{i=1}^N g(x; \xi_i)$$

$$\nabla \hat{\alpha}(x) = \frac{1}{N} \sum_{i=1}^N \nabla g(x; \xi_i)$$

↑
random
draws

Rollout acquisition

$$\alpha(x) = \mathbb{E}_{g \sim \text{posterior}_{\text{GP}}} [\min_{\text{proj. } x_k} (g(x_k) - g(\hat{x}))]$$

where \hat{x} is the best known sample point (before this)

Trajectory (for g)

$x_0 = x$ (starting point $\alpha(x)$)

$x_{k+1} = \underset{x}{\operatorname{argmax}} EI(x \mid \text{prior data up thru } k)$

?

$x \quad \dots \quad x_{-2} \quad x_{-1}$	x_0	$x_1 \quad x_2 \quad \dots \quad x_r$
<u>stuff</u>		<u>fantasized samples</u>
I've seen (known fn vals)		(guess values via a draw)

f unknown fn, assumed drawn from GP

Have sampled

x_{-m}, \dots, x_{-1} & got
 $y_{-m}, \dots, y_{-1}, y_j = f(x_j)$

Posterior dist \mathcal{G} , gaussian proc conditioned on samples at x_{-m}, \dots, x_{-1}

$$\alpha(x | g) = \max_{x_1, \dots, x_r} [g(x_k) - y_*]_+$$

x_1, \dots, x_r depend on g & hist
define by

$$x_{k+1} = \operatorname{argmax}_x EI(x | \text{samples through } x_k)$$

$$\alpha(x) = \mathbb{E}_{g \sim \mathcal{G}} [\alpha(x | g)]$$

$$\hat{\alpha}(x) = \frac{1}{N} \sum_{i=1}^N \alpha(x | g^i), \quad g^i \sim \mathcal{G} \text{ are draws}$$

To est deriv,

$$\nabla \hat{\alpha}(x) = \frac{1}{N} \sum_{i=1}^N \nabla \alpha(x | g^i)$$

Assume x_0 is unique best pt on trajectory for $x_0 = x$ & fn g^i
Then we want

$$\nabla [g(x_0) - y_*]$$

$$x_{k+1} = \underset{x}{\operatorname{argmax}} EI(x \mid x_{-m}, \dots, x_k, y_{-m}, \dots, y_k, g)$$

Stationarity: x_{k+1} solves

$$\nabla_x EI(x \mid x_{-m}, \dots, x_k, g) = 0$$

Solution to this is an implicitly defined function)

$$x_{k+1}(x_{-m}, \dots, x_k, g)$$

Get:

$$\nabla^2 EI(x_{k+1} \mid \dots) \delta x_{k+1}$$

$$+ \sum_{j=-m}^k \frac{\partial}{\partial x_j} EI(x_k \mid x_{-m}, \dots, x_k, g) \delta x_k$$

Algebra! And we have

$$\delta x_b = \frac{\partial x_b}{\partial x_0 = x}$$

$$\nabla d(x \mid g) = g'(x_b) \frac{\partial x_b}{\partial x_0}$$